Define ccExp

Launchbury/CoCallAnalysisImpl.thy
@@ -5,6 +5,14 @@ begin
 fun combined_restrict :: "var set \<Rightarrow> (AEnv \<times> CoCalls) \<Rightarrow> (AEnv \<times> CoCalls)"
   where "combined_restrict S (env, G) = (env f|` S, cc_restr S G)"
 
+lemma fst_combined_restrict[simp]:
+  "fst (combined_restrict S p) = fst p f|` S"
+  by (cases p, simp)
+
+lemma snd_combined_restrict[simp]:
+  "snd (combined_restrict S p) = cc_restr S (snd p)"
+  by (cases p, simp)
+
 lemma combined_restrict_eqvt[eqvt]:
   shows "\<pi> \<bullet> combined_restrict S p = combined_restrict (\<pi> \<bullet> S) (\<pi> \<bullet> p)"
   by (cases p) auto
@@ -32,13 +40,53 @@ proof(cases p)
   ultimately
   show ?thesis by simp
 qed
+
+definition predCC :: "var set \<Rightarrow> (Arity \<rightarrow> CoCalls) \<Rightarrow> (Arity \<rightarrow> CoCalls)"
+  where "predCC S f = (\<Lambda> a. if a \<noteq> 0 then cc_restr S (f\<cdot>(pred\<cdot>a)) else ccSquare S)"
+
+lemma predCC_eq:
+  shows "predCC S f \<cdot> a = (if a \<noteq> 0 then cc_restr S (f\<cdot>(pred\<cdot>a)) else ccSquare S)"
+  unfolding predCC_def
+  apply (rule beta_cfun)
+  apply (rule cont_if_else_above)
+  apply (auto dest: set_mp[OF ccFieldd_cc_restr])
+  done
+
+lemma predCC_eqvt[eqvt, simp]: "\<pi> \<bullet> (predCC S f) = predCC (\<pi> \<bullet> S) (\<pi> \<bullet> f)"
+  unfolding predCC_def
+  apply perm_simp
+  apply (rule Abs_cfun_eqvt)
+  apply (rule cont_if_else_above)
+  apply (auto dest: set_mp[OF ccFieldd_cc_restr])
+  done
+
+lemma cc_restr_usless[simp]:
+  "ccField G \<subseteq> S \<Longrightarrow> cc_restr S G = G"
+  apply transfer
+  apply (auto simp add: Field_def)
+  apply (metis Domain.DomainI contra_subsetD)
+  apply (metis Range.intros subsetCE)
+  done
+
+lemma cc_restr_cc_restr[simp]:
+  "cc_restr S (cc_restr S G) = cc_restr S G"
+  by transfer auto
+
+lemma cc_restr_cc_square[simp]:
+  "cc_restr S (ccSquare S) = ccSquare S"
+  by simp
+
+lemma cc_restr_predCC[simp]:
+  "cc_restr S (predCC S f\<cdot>n) = predCC S f\<cdot>n"
+  unfolding predCC_eq by simp
+
   
 nominal_function
   cccExp :: "exp \<Rightarrow> (Arity \<rightarrow> AEnv \<times> CoCalls)" 
 where
   "cccExp (GVar b x) = (\<Lambda> n . (AE_singleton x \<cdot> (up \<cdot> n), \<bottom>))"
-| "cccExp (Lam [x]. e) = (\<Lambda> n . combined_restrict (fv (Lam [x]. e)) (fst (cccExp e\<cdot>(pred\<cdot>n)), \<bottom>))"
-| "cccExp (App e x) = (\<Lambda> n . (fst (cccExp e\<cdot>(inc\<cdot>n)) \<squnion> (AE_singleton x \<cdot> (up \<cdot> 0)), \<bottom>))"
+| "cccExp (Lam [x]. e) = (\<Lambda> n . combined_restrict (fv (Lam [x]. e)) (fst (cccExp e\<cdot>(pred\<cdot>n)), predCC (fv (Lam [x]. e)) (\<Lambda> a. snd(cccExp e\<cdot>a))\<cdot>n))"
+| "cccExp (App e x) = (\<Lambda> n . (fst (cccExp e\<cdot>(inc\<cdot>n)) \<squnion> (AE_singleton x \<cdot> (up \<cdot> 0)), snd (cccExp e\<cdot>(inc\<cdot>n)) \<squnion> ccProd (fv e) {x}))"
 | "cccExp (Let as e) = (\<Lambda> n . combined_restrict (fv (Let as e)) (CoCallArityAnalysis.ccFix cccExp as \<cdot> (cccExp e \<cdot> n)))"
 proof-
 case goal1
@@ -52,20 +100,23 @@ next
 case goal3 thus ?case by (metis Terms.exp_strong_exhaust)
 next
 case (goal8 x e x' e')
-  from goal8(5)
+  from goal8(9)
   show ?case
   proof(rule eqvt_lam_case)
     fix \<pi> :: perm
     assume *: "supp (-\<pi>) \<sharp>* (fv (Lam [x]. e) :: var set)" 
     {
     fix n
-    have "combined_restrict (fv (Lam [x]. e)) (fst (cccExp_sumC (\<pi> \<bullet> e)\<cdot>(pred\<cdot>n)), \<bottom>) = combined_restrict (fv (Lam [x]. e)) (- \<pi> \<bullet> (fst (cccExp_sumC (\<pi> \<bullet> e)\<cdot>(pred\<cdot>n)), \<bottom>))"
+    have "combined_restrict (fv (Lam [x]. e)) (fst (cccExp_sumC (\<pi> \<bullet> e)\<cdot>(pred\<cdot>n)), predCC (fv (Lam [x]. e)) (\<Lambda> a. snd(cccExp_sumC (\<pi> \<bullet> e)\<cdot>a))\<cdot>n)
+       = combined_restrict (fv (Lam [x]. e)) (- \<pi> \<bullet> (fst (cccExp_sumC (\<pi> \<bullet> e)\<cdot>(pred\<cdot>n)), predCC (fv (Lam [x]. e)) (\<Lambda> a. snd(cccExp_sumC (\<pi> \<bullet> e)\<cdot>a))\<cdot>n))"
       by (rule combined_restrict_perm[symmetric, OF *]) simp
-    also have "\<dots> = combined_restrict (fv (Lam [x]. e)) (fst (cccExp_sumC e\<cdot>(pred\<cdot>n)), \<bottom>)"
-      by (simp add: eqvt_at_apply[OF goal8(1)] pemute_minus_self)
+    also have "\<dots> = combined_restrict (fv (Lam [x]. e)) (fst (cccExp_sumC e\<cdot>(pred\<cdot>n)), predCC (- \<pi> \<bullet> fv (Lam [x]. e)) (\<Lambda> a. snd(cccExp_sumC e\<cdot>a))\<cdot>n)"
+      by (perm_simp, simp add: eqvt_at_apply[OF goal8(1)] pemute_minus_self Abs_cfun_eqvt)
+    also have "- \<pi> \<bullet> fv (Lam [x]. e) = (fv (Lam [x]. e) :: var set)" by (rule perm_supp_eq[OF *])
     also note calculation
     }
-    thus "(\<Lambda> n. combined_restrict (fv (Lam [x]. e)) (fst (cccExp_sumC (\<pi> \<bullet> e)\<cdot>(pred\<cdot>n)), \<bottom>)) = (\<Lambda> n. combined_restrict (fv (Lam [x]. e)) (fst (cccExp_sumC e\<cdot>(pred\<cdot>n)), \<bottom>))" by simp
+    thus "(\<Lambda> n. combined_restrict (fv (Lam [x]. e)) (fst (cccExp_sumC (\<pi> \<bullet> e)\<cdot>(pred\<cdot>n)), predCC (fv (Lam [x]. e)) (\<Lambda> a. snd(cccExp_sumC (\<pi> \<bullet> e)\<cdot>a))\<cdot>n))
+        = (\<Lambda> n. combined_restrict (fv (Lam [x]. e)) (fst (cccExp_sumC e\<cdot>(pred\<cdot>n)), predCC (fv (Lam [x]. e)) (\<Lambda> a. snd(cccExp_sumC e\<cdot>a))\<cdot>n))" by simp
   qed
 next
 case (goal13 as body as' body')
@@ -94,6 +145,26 @@ case (goal13 as body as' body')
 qed auto
 
 nominal_termination (eqvt) by lexicographic_order
+
+interpretation CoCallArityAnalysis cccExp.
+
+definition aExp :: "exp \<Rightarrow> (Arity \<rightarrow> AEnv)" where "aExp e = (\<Lambda> a. fst (cccExp e \<cdot> a))"
+lemma aExp_simps:
+  "aExp (GVar b x)\<cdot>n = AE_singleton x\<cdot>(up\<cdot>n)"
+  "aExp (Lam [x]. e)\<cdot>n = aExp e\<cdot>(pred\<cdot>n) f|` fv (Lam [x]. e)"
+  "aExp (App e x)\<cdot>n = aExp e\<cdot>(inc\<cdot>n) \<squnion> AE_singleton x\<cdot>(up\<cdot>0)"
+  "aExp (Let as e)\<cdot>n = fst (ccFix as\<cdot>(cccExp e \<cdot> n)) f|` fv (Let as e)"
+unfolding aExp_def by (simp add: beta_cfun)+
+
+
+definition ccExp :: "exp \<Rightarrow> (Arity \<rightarrow> CoCalls)" where "ccExp e = (\<Lambda> a. snd (cccExp e \<cdot> a))"
+lemma ccExp_simps:
+  "ccExp (GVar b x)\<cdot>n = \<bottom>"
+  "ccExp (Lam [x]. e)\<cdot>n = predCC (fv (Lam [x]. e)) (ccExp e)\<cdot>n"
+  "ccExp (App e x)\<cdot>n = ccExp e\<cdot>(inc\<cdot>n) \<squnion> ccProd (fv e) {x}"
+  "ccExp (Let as e)\<cdot>n = cc_restr (fv (Let as e)) (snd (ccFix as\<cdot>(cccExp e\<cdot>n)))"
+unfolding ccExp_def by (simp add: beta_cfun)+
+
 
 end
 
